Add LL(1) derivation relation and a proof that it's deterministic for LL(1) grammars

LL1/DeterminismWalkthrough.v
@@ -780,9 +780,14 @@ Proof.
     + (* We can't prove this append fact, so we're stuck *)
 Abort.
 
-(* In this attempt, I try to prove that each symbol on the
-   right-hand side of a production and the symbols to its
-   right can only split the input in one way. *)
+Fixpoint inF tr f :=
+  match f with
+  | Fnil => False
+  | Fcons tr' f' => tr = tr' \/ inF tr f'
+  end.
+
+
+
 Lemma derives_det :
   forall tbl g,
     isParseTableFor tbl g
@@ -802,27 +807,704 @@ Proof.
   intros tbl g Htbl.
   pose proof Htbl as Htbl'.
   destruct Htbl as [Hmin Hcom].
+  induction tr using tree_nested_ind with
+      (Q := fun f =>
+              forall x gpre gsuf word,
+                In (x, gpre ++ gsuf) (productions g)
+                -> derivesForest gsuf word f
+                -> forall tr tr' sym w,
+                    inF tr f
+                    -> derivesTree sym w tr
+                    -> derivesTree sym w tr'
+                    -> tr = tr); intros.
+
+  - inv H0.
+    inv H1.
+    assert (
+    
   induction tr using tree_mutual_ind with
-      (P0 := fun fsuf =>
-               forall fsuf' x gpre gsuf
+      (P0 := fun f =>
+               (forall f' x gpre sym gsuf
                       wpre wpre' wsuf wsuf'
-                      fpre fpre',
-                 In (x, gpre ++ gsuf) (productions g)
-                 -> derivesForest gpre wpre fpre
-                 -> derivesForest gpre wpre' fpre'
-                 -> derivesForest gsuf wsuf fsuf
-                 -> derivesForest gsuf wsuf' fsuf'
+                      tr tr',
+                 In (x, gpre ++ sym :: gsuf) (productions g)
+                 -> derivesTree sym wpre tr
+                 -> derivesTree sym wpre' tr'
+                 -> derivesForest gsuf wsuf f
+                 -> derivesForest gsuf wsuf' f'
                  -> wpre ++ wsuf = wpre' ++ wsuf'
                  -> wpre = wpre'
                     /\ wsuf = wsuf'
-                    /\ fsuf = fsuf'); intros.
-  
+                    /\ fsuf = fsuf')
+               /\ (forall f' lx gpre rx gsuf gsuf2,
+                      In (lx, gpre ++ NT rx :: gsuf)
+                         (productions g)
+                      -> derivesForest gsuf2 wpre f
+                      -> derivesForest gsuf2 wpre' f'
+                      -> derivesForest gsuf wsuf fsuf
+                      -> derivesForest gsuf wsuf' fsuf'
+                      -> wpre ++ wsuf = wpre' ++ wsuf'
+                      -> wpre = wpre' /\ wsuf = wsuf' /\
+                         fsuf = fsuf')
+
+               ; intros.
+  - inv H0; inv H1; inv H4; auto.
   - inv H0; inv H1.
-    inv H4.
+    assert (gamma0 = gamma) by admit; subst.
+    
+
+
+
+
+
+Inductive ForallF (P : tree -> Prop) : forest -> Prop :=
+| ForallFnil : ForallF P Fnil
+| ForallFcons : forall tr f',
+    P tr -> ForallF P f' -> ForallF P (Fcons tr f').
+
+Inductive tree_det {g : grammar} :
+  symbol -> list string -> tree -> Prop :=
+| Leaf_det :
+    forall y word,
+    (forall word' tr',
+        (@derivesTree g) (T y) word (Leaf y)
+        -> (@derivesTree g) (T y) word' tr'
+        -> word = word')
+    -> tree_det (T y) word (Leaf y)
+| Node_det :
+    forall x gamma word f,
+      In (x, gamma) (productions g)
+      -> forest_det gamma word f
+      -> tree_det (NT x) word (Node x f)
+with forest_det {g : grammar} :
+        list symbol -> list string -> forest -> Prop :=
+     | Fnil_det :
+         forest_det nil nil Fnil
+     | Fcons_det :
+         forall hd tl wpre wsuf tr f,
+           tree_det hd wpre tr
+           -> forest_det tl wsuf f
+           -> (forall wpre' wsuf' tr' f',
+                  wpre ++ wsuf = wpre' ++ wsuf'
+                  -> (@derivesTree g) hd wpre tr
+                  -> (@derivesTree g) hd wpre' tr'
+                  -> (@derivesForest g) tl wsuf f
+                  -> (@derivesForest g) tl wsuf' f'
+                  -> wpre = wpre'
+                     /\ wsuf = wsuf')
+           -> forest_det (hd :: tl) (wpre ++ wsuf) (Fcons tr f).
+
+Lemma ll1_det :
+  forall tbl g,
+    isParseTableFor tbl g
+    -> forall tr sym word,
+      (@derivesTree g) sym word tr
+      -> (@tree_det g) sym word tr.
+Proof.
+  intros tbl g Htbl.
+  induction tr using tree_mutual_ind with
+      (P := fun tr =>
+              forall sym word,
+                (@derivesTree g) sym word tr
+                -> (@tree_det g) sym word tr)
+      (P0 := fun f =>
+               forall x gpre gsuf word,
+                 In (x, gpre ++ gsuf) (productions g)
+                 -> derivesForest gsuf word f
+                 -> (@forest_det g) gsuf word f); intros.
+
+  - inv H.
+    constructor; intros.
+    inv H0.
+    auto.
+  - inv H.
+    econstructor; intros; eauto.
+    eapply IHtr with (gpre := nil); eauto.
+  - inv H0.
+    constructor.
+  - inv H0.
+    constructor; intros.
+    + eapply IHtr; auto.
+    + eapply IHtr0 with (gpre := gpre ++ [hdRoot]); eauto.
+      admit.
+    + eapply IHtr in H5.
+      
+    constructor.
+               forall 
+              forall x gpre sym gsuf wpre wsuf fsuf,
+                In (x, gpre ++ sym :: gsuf) (productions g)
+                -> (@derivesTree g) sym wpre tr
+                -> (@derivesForest g) gsuf wsuf fsuf
+                -> (@tree_det g) tr)
+      (P0 := fun f =>
+               forall x gpre gsuf word,
+                 In (x, gpre ++ gsuf) (productions g)
+                 -> derivesForest gsuf word f
+                 -> (@forest_det g) f); intros.
+
+  - inv H0.
+    econstructor; intros; constructor; auto.
+  - inv H0.
+    constructor; intros.
+    + eapply IHtr with (gpre := nil); eauto.
+    + assert (gamma0 = gamma') by admit; 
+
+
+    constructor.
+  - inv H.
+    constructor; intros.
+    + eapply IHtr with (gpre := nil); eauto.
+    + admit.
+  - constructor.
+  - inv H0.
+    constructor; intros.
+    + eapply IHtr; eauto.
+    + eapply IHtr0 with (gpre := gpre ++ [hdRoot]); eauto.
+      assert (hdRoot :: tlRoots = [hdRoot] ++ tlRoots) by auto.
+      rewrite H0 in H.
+      rewrite app_assoc in H.
+      eauto.
+    + induction gpre.
+      * eapply IHtr0 with (gpre := gpre ++ [hdRoot]) in H6;
+        eauto.
+      * inv H6.
+        -- inv H3; inv H4.
+           repeat rewrite app_nil_r in *.
+           auto.
+        -- inv H3; inv H4.
+
+          
+      assert (hdRoot :: tlRoots = [hdRoot] ++ tlRoots) by auto.
+      rewrite H0 in H.
+      rewrite app_assoc in H.
+      eauto.eapply IHtr0 in 
+
+
+
+
+
+
+
+
+
+
+
+
+
+
+
+
+      
+
+Inductive tree_det' {g : grammar} :
+  tree -> Prop :=
+| Leaf_det' :
+    forall y,
+      tree_det' (Leaf y)
+| Node_det' :
+    forall x f,
+      forest_det' f
+      -> (forall lx f' gamma gamma' wpre wpre' wsuf wsuf'
+             fsuf fsuf' gpre gsuf,
+             In (lx, gpre ++ NT x :: gsuf) (productions g)
+             -> In (x, gamma) (productions g)
+             -> In (x, gamma') (productions g)
+             -> (@derivesForest g) gamma wpre f
+             -> (@derivesForest g) gamma' wpre' f'
+             -> (@derivesForest g) gsuf wsuf fsuf
+             -> (@derivesForest g) gsuf wsuf' fsuf'
+             -> wpre ++ wsuf = wpre' ++ wsuf'
+             -> gamma = gamma' /\ wpre = wpre' /\ wsuf = wsuf')
+      -> tree_det' (Node x f)
+with forest_det' {g : grammar} :
+       forest -> Prop :=
+     | Fnil_det' : forest_det' Fnil
+     | Fcons_det' :
+         forall tr f,
+           tree_det' tr
+           -> forest_det' f
+           -> (forall hd tl wpre wpre' wsuf wsuf' tr' f',
+                  wpre ++ wsuf = wpre' ++ wsuf'
+                  -> (@derivesTree g) hd wpre tr
+                  -> (@derivesTree g) hd wpre' tr'
+                  -> (@derivesForest g) tl wsuf f
+                  -> (@derivesForest g) tl wsuf' f'
+                  -> wpre = wpre'
+                     /\ wsuf = wsuf')
+           -> forest_det' (Fcons tr f).
+
+Lemma ll1_det :
+  forall tbl g,
+    isParseTableFor tbl g
+    -> forall tr sym word,
+      (@derivesTree g) sym word tr
+      -> (@tree_det' g) tr.
+Proof.
+  intros tbl g Htbl.
+  induction tr using tree_mutual_ind with
+      (P := fun tr =>
+              forall sym word,
+              derivesTree sym word tr -> tree_det' tr)
+      (P0 := fun f =>
+               forall x gpre gsuf word,
+                 In (x, gpre ++ gsuf) (productions g)
+                 -> derivesForest gsuf word f ->
+                 forest_det' f); intros.
+  - constructor.
+  - inv H.
+    constructor; intros.
+    + eapply IHtr with (gpre := nil) ; eauto.
+    + assert (gamma0 = gamma') by admit.
+      subst.
+      
+
+
+
+
+
+
+  
+
+Definition tree_det' {g : grammar} tr :=
+  forall sym word tr',
+    (@derivesTree g) sym word tr
+    -> (@derivesTree g) sym word tr'
+    -> tr = tr'.
+
+Definition forest_det' {g : grammar} f :=
+  forall gamma word f',
+    (@derivesForest g) gamma word f
+    -> (@derivesForest g) gamma word f'
+    -> f = f'.
+
+Lemma det_det' :
+  forall g tr,
+    (@tree_det g) tr -> (@tree_det' g) tr.
+Proof.
+  intros g.
+  induction tr using tree_mutual_ind with
+      (P := fun tr => (@tree_det g) tr -> (@tree_det' g) tr)
+      (P0 := fun f => (@forest_det g) f -> (@forest_det' g) f)
+  ; intros.
+  - unfold tree_det'; intros.
+    inv H0; inv H1; auto.
+  - inv H.
+    unfold tree_det'; intros.
+    inv H; inv H0.
+    pose proof H4 as H4'.
+    eapply H3 with (gamma := gamma) in H4; eauto; subst.
+    apply IHtr in H2.
+    unfold forest_det' in H2.
+    erewrite H2; eauto.
+  - unfold forest_det'; intros.
+    inv H0; inv H1; auto.
+  - inv H.
+    unfold forest_det'; intros.
+    inv H; inv H0.
+    pose proof H10 as H10'.
+    eapply H4 with (wpre := prefix)
+                   (wsuf := suffix) in H10; eauto.
+    destruct H10; subst.
+    eapply IHtr in H2.
+    unfold tree_det' in H2.
+    erewrite H2; eauto.
+    eapply IHtr0 in H3.
+    unfold forest_det' in H3.
+    erewrite H3; eauto.
+Qed.
+    
+Section list_length_ind.  
+  Variable A : Type.
+  Variable P : list A -> Prop.
+
+  Hypothesis H : forall xs, (forall l, List.length l < List.length xs -> P l) -> P xs.
+
+  Theorem list_length_ind : forall xs, P xs.
+  Proof.
+    assert (forall xs l : list A, List.length l <= List.length xs -> P l) as H_ind.
+    { induction xs; intros l Hlen; apply H; intros l0 H0.
+      - inversion Hlen. omega.
+      - apply IHxs. simpl in Hlen. omega.
+    }
+    intros xs.
+    apply H_ind with (xs := xs).
+    omega.
+  Qed.
+End list_length_ind.
+
+
+              
+            
+
+
+(*
+Inductive symbol_det {g : grammar} :
+  symbol -> Prop :=
+| T_det :
+  forall y word word' tr tr',
+    (@derivesTree g) (T y) word tr
+    -> (@derivesTree g) (T y) word' tr'
+    -> word = word' /\ tr = tr'
+    -> symbol_det (T y)
+| NT_det :
+    forall x,
+      (forall gamma gamma' word f f',
+          In (x, gamma) (productions g)
+          -> In (x, gamma') (productions g)
+          -> (@derivesForest g) gamma word f
+          -> (@derivesForest g) gamma' word f'
+          -> gamma = gamma' /\ f = f' /\ gamma_det gamma)
+    -> symbol_det (NT x)
+with gamma_det {g : grammar} :
+       list symbol -> Prop :=
+     | Fnil_det : gamma_det nil
+     | Fcons_dfp :
+         forall hd tl wpre wpre' wsuf wsuf' tr tr' f f',
+           symbol_det hd
+           -> gamma_det tl
+           -> wpre ++ wsuf = wpre' ++ wsuf'
+           -> (@derivesTree g) hd wpre tr
+           -> (@derivesTree g) hd wpre' tr'
+           -> (@derivesForest g) tl wsuf f
+           -> (@derivesForest g) tl wsuf' f'
+           -> wpre = wpre'
+              /\ wsuf = wsuf'
+              /\ tr = tr'
+              /\ f = f'
+           -> gamma_det (hd :: tl).
+ *)
+
+Scheme symbol_det_mutual_ind :=
+  Induction for symbol_det Sort Prop
+  with gamma_det_mutual_ind := Induction for gamma_det Sort Prop.
+
+Inductive symbol_det' {g : grammar} :
+  symbol -> Prop :=
+| T_det' :
+    forall y word word' tr tr',
+      (@derivesTree g) (T y) word tr
+      -> (@derivesTree g) (T y) word' tr'
+      -> word = word' /\ tr = tr'
+      -> symbol_det' (T y)
+| NT_det' :
+    forall x,
+      (forall gamma gamma' word f f',
+          In (x, gamma) (productions g)
+          -> In (x, gamma') (productions g)
+          -> (@derivesForest g) gamma word f
+          -> (@derivesForest g) gamma' word f'
+          -> gamma = gamma' /\ f = f')
+      -> symbol_det' (NT x).
+
+
+Definition symbol_det'' {g : grammar} sym :=
+  forall word tr tr',
+    (@derivesTree g) sym word tr
+    -> (@derivesTree g) sym word tr'
+    -> tr = tr'.
+
+
+Lemma det_det' :
+  forall g sym,
+    (@symbol_det g) sym -> (@symbol_det' g) sym.
+Proof.
+  intros g sym.
+  induction 1 using symbol_det_mutual_ind.
+  - econstructor; eauto.
+  - econstructor; intros.
+    eapply a with (gamma := gamma) (f := f) in H2; eauto.
+    destruct H2.
+    destruct H3.
+    split; auto.
+Qed.
+
+Lemma det'_det'' :
+  forall g sym,
+    (@symbol_det' g) sym -> (@symbol_det'' g) sym.
+Proof.
+  induction 1; intros.
+  - unfold symbol_det''; intros.
+    inv H2; inv H3; auto.
+  - unfold symbol_det''; intros.
+    inv H0; inv H1.
+    eapply H with
+        (gamma := gamma) (f := subtrees) in H5; eauto.
+    destruct H5.
+    subst; auto.
+Qed.
+
+Lemma det_det'' :
+  forall g sym,
+    (@symbol_det g) sym -> (@symbol_det'' g) sym.
+Proof.
+  intros.
+  apply det'_det''.
+  apply det_det'.
+  auto.
+Qed.
+
+Lemma ll1_det :
+  forall tbl g,
+    isParseTableFor tbl g
+    -> forall sym,
+      (@derivesTree 
+      (@symbol_det g) sym.
+Proof.
+  destruct sym
+
+  
+  induction sym.
+  - admit.
+  - 
+  destruct sym as [y | x].
+  - econstructor; eauto.
+    + constructor.
+    + constructor.
+  - econstructor; intros.
+    assert (gamma' = gamma) by admit; subst.
+    induction gamma.
+    + inv H2; inv H3.
+      repeat (split; auto).
+      constructor.
+    + 
+  
+
+    
+                
+    
+                    
+
+Inductive symbol_dfp {g : grammar} :
+  symbol -> Prop :=
+| T_dfp :
+  forall y wpre wpre' wsuf wsuf' tr tr',
+    (@derivesTree g) (T y) wpre tr
+    -> (@derivesTree g) (T y) wpre' tr'
+    -> wpre ++ wsuf = wpre' ++ wsuf
+    -> wpre = wpre' /\ wsuf = wsuf'
+    -> symbol_dfp (T y)
+| NT_dfp :
+    forall x gamma,
+      In (x, gamma) (productions g)
+      -> gamma_dfp gamma
+      -> symbol_dfp (NT x)
+with gamma_dfp {g : grammar} :
+       list symbol -> Prop :=
+     | Fnil_dfp : gamma_dfp nil
+     | Fcons_dfp :
+         forall sym syms,
+           symbol_dfp sym
+           -> gamma_dfp syms
+           -> gamma_dfp (sym :: syms).
+
+Scheme symbol_dfp_ind' := Induction for symbol_dfp Sort Prop
+  with gamma_dfp_ind' := Induction for gamma_dfp Sort Prop.
+
+Lemma dfp :
+  forall g sym,
+    (@symbol_dfp g) sym
+    -> forall x gpre gsuf wpre wpre' wsuf wsuf' tr tr'
+              fsuf fsuf',
+      In (x, gpre ++ sym :: gsuf) (productions g)
+      -> (@derivesTree g) sym wpre tr
+      -> (@derivesTree g) sym wpre' tr'
+      -> (@derivesForest g) gsuf wsuf fsuf
+      -> (@derivesForest g) gsuf wsuf' fsuf'
+      -> wpre ++ wsuf = wpre' ++ wsuf'
+      -> wpre = wpre' /\ wsuf = wsuf'.
+Proof.
+  intros g sym.
+  induction 1 using symbol_dfp_ind' with
+      (P := fun sym (pf : symbol_dfp sym) =>
+              forall x gpre gsuf wpre wpre' wsuf wsuf' tr tr'
+                     fsuf fsuf',
+                In (x, gpre ++ sym :: gsuf) (productions g)
+                -> (@derivesTree g) sym wpre tr
+                -> (@derivesTree g) sym wpre' tr'
+                -> (@derivesForest g) gsuf wsuf fsuf
+                -> (@derivesForest g) gsuf wsuf' fsuf'
+                -> wpre ++ wsuf = wpre' ++ wsuf'
+                -> wpre = wpre' /\ wsuf = wsuf')
+      (P0 := fun gamma (pf : gamma_dfp gamma) =>
+               forall wpre wpre' wsuf wsuf' f f',
+                (@derivesForest g) gamma wpre f
+                -> (@derivesForest g) gamma wpre' f'
+                -> wpre ++ wsuf = wpre' ++ wsuf'
+                -> wpre = wpre' /\ wsuf = wsuf'); intros.
+
+  - inv H0; inv H1; inv H4.
+    split; auto.
+
+  - inv H0; inv H1.
+    assert (gamma0 = gamma1) by admit.
+    subst.
+    inv g0.
+    
+  
+
+Lemma dfp :
+  forall tbl g,
+    isParseTableFor tbl g
+    -> forall tr x gpre sym gsuf wpre wsuf fsuf,
+      In (x, gpre ++ sym :: gsuf) (productions g)
+      -> (@derivesTree g) sym wpre tr
+      -> (@derivesForest g) gsuf wsuf fsuf
+      -> (@symbol_dfp g) sym.
+Proof.
+  intros tbl g Htbl.
+  destruct Htbl as [Hmin Hcom].
+  induction tr using tree_mutual_ind with
+      (P := fun tr =>
+              forall x gpre sym gsuf wpre wsuf fsuf,
+                In (x, gpre ++ sym :: gsuf) (productions g)
+                -> (@derivesTree g) sym wpre tr
+                -> (@derivesForest g) gsuf wsuf fsuf
+                -> (@symbol_dfp g) sym)
+      (P0 := fun fsuf =>
+               forall x gpre gsuf word,
+                 In (x, gpre ++ gsuf) (productions g)
+                 -> (@derivesForest g) gsuf word fsuf
+                 -> (@gamma_dfp g) gsuf); intros.
+  - inv H0.
+    eapply T_dfp; constructor; auto.
+
+  - inv H0.
+    eapply NT_dfp; eauto.
+    eapply IHtr with (gpre := nil); eauto.
+
+  - inv H0.
+    constructor.
+
+  - inv H0.
+    eapply Fcons_dfp; eauto.
+    eapply IHtr0; eauto.
+    assert (hdRoot :: tlRoots = [hdRoot] ++ tlRoots) by auto.
+    rewrite H0 in H.
+    rewrite app_assoc in H.
+    eauto.
+    Unshelve.
+    auto.
+Qed.
+    
+Definition treeDerivesFixedPrefix (g : grammar) (tr : tree) :=
+  forall tr tr' sym wpre wpre' wsuf wsuf',
+    (@derivesTree g) sym wpre tr
+    -> (@derivesTree g) sym wpre' tr'
+    -> wpre ++ wsuf = wpre' ++ wsuf'
+    -> wpre = wpre'
+       /\ wsuf = wsuf'
+       /\ tr = tr'.
+
+Definition forestDerivesFixedPrefix g f :=
+  ForallF (treeDerivesFixedPrefix g) f.
+
+Lemma ForallF_derivesForest :
+  forall g f f' gamma wpre wpre' wsuf wsuf',
+    forestDerivesFixedPrefix g f
+    -> (@derivesForest g) gamma wpre f
+    -> (@derivesForest g) gamma wpre' f'
+    -> wpre ++ wsuf = wpre' ++ wsuf'
+    -> wpre = wpre' /\ wsuf = wsuf' /\ f = f'.
+Proof.
+  induction f; intros.
+  - inv H0; inv H1.
+    simpl in *.
+    repeat (split; auto).
+  - inv H; inv H0; inv H1.
+    eapply H5 with
+        (wpre := prefix)
+        (wpre' := prefix0)
+        (wsuf := suffix ++ wsuf)
+        (wsuf' := suffix0 ++ wsuf') in H3; eauto.
+    (* Not sure why that didn't give me prefix = prefix0 *)
+    + destruct H3.
+      subst.
+      eapply IHf in H10; eauto.
+      destruct H10.
+      destruct H1.
+      subst.
+      repeat apply prefixes_eq in H2; subst.
+      repeat (split; auto).
+    + repeat rewrite app_assoc. auto.
+Qed.
+
+Lemma derives_det :
+  forall tbl g,
+    isParseTableFor tbl g
+    -> forall tr tr' x gpre sym gsuf
+              wpre wpre' wsuf wsuf'
+              fsuf fsuf',
+      In (x, gpre ++ sym :: gsuf) (productions g)
+      -> (@derivesTree g) sym wpre tr
+      -> (@derivesTree g) sym wpre' tr'
+      -> (@derivesForest g) gsuf wsuf fsuf
+      -> (@derivesForest g) gsuf wsuf' fsuf'
+      -> wpre ++ wsuf = wpre' ++ wsuf'
+      -> treeDerivesFixedPrefix g tr.
+Proof.
+  intros tbl g Htbl.
+  pose proof Htbl as Htbl'.
+  destruct Htbl as [Hmin Hcom].
+  induction tr using tree_mutual_ind with
+      (P0 := fun fsuf =>
+               forall x gpre gsuf word,
+                 In (x, gpre ++ gsuf) (productions g)
+                 -> derivesForest gsuf word fsuf
+                 -> forestDerivesFixedPrefix g fsuf);
+    intros.
+  
+  - inv H0; inv H1; inv H4.
     repeat (split; auto).
 
   - inv H0; inv H1.
     assert (gamma0 = gamma) by admit; subst.
+    pose proof H9 as H9'.
+    eapply IHtr with (gpre := nil) in H9; eauto.
+    eapply ForallF_derivesForest in H9; eauto.
+    destruct H9.
+    destruct H1.
+    subst.
+    repeat (split; auto). 
+
+  - constructor.
+
+  - inv H0.
+    constructor.
+    + unfold derivesFixedPrefix; intros.
+      
+
+      eapply IHtr0 with
+          (gpre := gpre ++ [hdRoot]) in H6; eauto.
+      * unfold derivesFixedPrefix; intros.
+        
+
+      eapply IHtr in H6; eauto.
+    + eapply IHtr0 with
+          (gpre := gpre ++ [hdRoot]); eauto.
+      assert (hdRoot :: tlRoots = [hdRoot] ++ tlRoots) by auto.
+      rewrite H0 in H.
+      rewrite app_assoc in H.
+      eauto.
+    constructor.
+    + unfold derivesFixedPrefix; intros.
+      destruct tr as [y | rx].
+      * inv H0; inv H1; inv H2.
+        repeat (split; auto).
+      * inv H0.
+        inv H5.
+        inv H1.
+        
+      apply IHtr in 
+    + eapply IHtr0 with
+          (gpre := gpre ++ [hdRoot]); eauto.
+      assert (hdRoot :: tlRoots = [hdRoot] ++ tlRoots) by auto.
+      rewrite H0 in H.
+      rewrite app_assoc in H.
+      eauto.
+      
+
+
+    
     (* This is looking good, but if we try to apply IHtr
        to one of our other hypotheses, we run into trouble
        because it expects gpre and gsuf to appear in the
@@ -842,3 +1524,425 @@ Proof.
     + (* We can't prove this append fact, so we're stuck *)
 Abort.
 
+Lemma or_thing :
+  forall g tr tr' sym word,
+    (@derivesTree g) sym word tr
+    -> (@derivesTree g) sym word tr'
+    -> tr = tr'
+       \/ exists x gamma gamma' word' f f',
+        In (x, gamma) (productions g)
+        /\ In (x, gamma') (productions g)
+        /\ (@derivesForest g) gamma word' f
+        /\ (@derivesForest g) gamma' word' f'
+        /\ gamma <> gamma'.
+Proof.
+  intro g.
+  induction tr using tree_mutual_ind with
+      (P := fun tr => 
+              forall tr' sym word,
+                (@derivesTree g) sym word tr
+                -> (@derivesTree g) sym word tr'
+                -> tr = tr'
+                   \/ exists x gamma gamma' word' f f',
+                    In (x, gamma) (productions g)
+                    /\ In (x, gamma') (productions g)
+                    /\ (@derivesForest g) gamma word' f
+                    /\ (@derivesForest g) gamma' word' f'
+                    /\ gamma <> gamma')
+      (P0 := fun f =>
+               forall f' gamma word,
+                 (@derivesForest g) gamma word f
+                 -> (@derivesForest g) gamma word f'
+                 -> f = f'
+                    \/ exists x gamma gamma' word' f f',
+                     In (x, gamma) (productions g)
+                     /\ In (x, gamma') (productions g)
+                     /\ (@derivesForest g) gamma word' f
+                     /\ (@derivesForest g) gamma' word' f'
+                     /\ gamma <> gamma'); intros.
+  - inv H; inv H0.
+    left; auto.
+
+  - inv H; inv H0.
+    destruct (list_eq_dec symbol_eq_dec gamma0 gamma).
+    + subst.
+      apply IHtr in H2; auto.
+      destruct H2.
+      * subst.
+        left; auto.
+      * right.
+        auto.
+    + right.
+      exists s; exists gamma; exists gamma0; exists word;
+        exists f; exists subtrees.
+      repeat (split; auto).
+
+  - inv H; inv H0.
+    left; auto.
+
+  - inv H; inv H0.
+    destruct (list_eq_dec string_dec prefix prefix0).
+    + subst.
+      apply suffixes_eq in H2.
+      subst.
+      apply IHtr in H3; auto.
+Abort.
+
+Lemma even_splits :
+  forall tbl g,
+    isParseTableFor tbl g
+    -> forall wsuf gsuf x gpre wpre wpre' wsuf' fsuf fsuf',
+      In (x, gpre ++ gsuf) (productions g)
+      -> (@derivesForest g) gsuf wsuf fsuf
+      -> (@derivesForest g) gsuf wsuf' fsuf'
+      -> wpre ++ wsuf = wpre' ++ wsuf'
+      -> wpre = wpre'
+         /\ wsuf = wsuf'.
+Proof.
+  intros tbl g Htbl.
+  induction wsuf as [| stok stoks]; intros.
+  - rewrite app_nil_r in *.
+    subst.
+    admit.
+  - 
+    
+Abort.
+
+
+(* IN THIS SECTION, I'M TRYING TO PROVE THAT AN LL(1) 
+   DERIVATION TREE MUST SPLIT THE INPUT DETERMINISTICALLY,
+   WITHOUT WORRYING ABOUT TREE STRUCTURE *)
+
+Fixpoint size tr :=
+  match tr with
+  | Leaf _ => 0
+  | Node _ f => S (sizeForest f)
+  end
+with sizeForest f :=
+       match f with
+       | Fnil => 0
+       | Fcons tr f' => size tr + sizeForest f'
+       end.
+
+Lemma nat_strong_ind: forall (P:nat -> Prop),
+P 0 -> (forall n:nat, (forall (m:nat), m <= n -> P m) -> P (S n)) -> forall n, P n.
+Proof.
+intros P B IHs n.
+destruct n.
+exact B.
+apply IHs.
+induction n.
+intros m H; replace m with 0; try omega; exact B.
+intros m H.
+assert (m <= n \/ m = S n) as J; try omega.
+destruct J as [J|J].
+apply IHn; omega.
+rewrite J.
+apply IHs. 
+apply IHn.
+Qed.
+
+Lemma length_nil: forall A:Type, forall l:list A, 
+  l = nil <-> List.length l = 0.
+Proof.
+split; intros H.
+rewrite H; simpl; auto.
+destruct l. auto.
+contradict H; simpl.
+apply sym_not_eq; apply O_S.
+Qed.
+
+Lemma length_strong_ind: forall (A:Type) (P:list A -> Prop),
+P nil -> (forall (n:nat) (k:list A), (forall (l:list A), List.length l <= n -> P l) -> List.length k = S n -> P k) -> forall l, P l.
+Proof.
+intros A P B IH.
+assert (forall (n:nat) (l:list A), List.length l <= n -> P l) as G.
+intro n.
+induction n as [| n IHS] using nat_strong_ind.
+intros l H.
+assert (List.length l = 0) as G; try omega.
+apply length_nil in G.
+rewrite G; exact B.
+intro l.
+intro H.
+assert (List.length l <= n \/ List.length l = S n) as G; try omega.
+destruct G as [G|G].
+apply IHS with (m:=n); auto.
+apply IH with (n:=n); try exact G.
+intro k.
+apply IHS with (m:=n) (l:=k).
+auto.
+intro l.
+apply G with (n:=List.length l); auto.
+Qed.
+
+(* EACH TREE/SYMBOL STRIPS AWAY JUST ONE PREFIX *)
+
+Lemma derives_det :
+  forall tbl g,
+    isParseTableFor tbl g
+    -> forall word tr tr' sym,
+      (@derivesTree g) sym word tr
+      -> (@derivesTree g) sym word tr'
+      -> tr = tr'.
+Proof.
+  intros tbl g Htbl.
+  pose proof Htbl as Htbl'.
+  destruct Htbl as [Hmin Hcom].
+  intro word.
+  induction word using length_strong_ind; intros.
+  - destruct sym.
+    + inv H.
+    + inv H.
+      inv H0.
+      admit.
+  - destruct sym.
+    + inv H1; inv H2.
+      auto.
+    + inv H1.
+      inv H2.
+  
+  induction tr using tree_mutual_ind with
+      (P0 := fun f =>
+               forall f' gamma word,
+                 (@derivesForest g) gamma word f
+                 -> (@derivesForest g) gamma word f'
+                 -> f = f'); intros.
+  
+
+(* Maybe do induction on wsuf *)
+Lemma rosenkrantz_lemma_4'' :
+  forall tbl g,
+    isParseTableFor tbl g
+    -> forall word wmid lx gpre rx gamma gsuf
+              wsuf
+              fmid fsuf,
+      In (lx, gpre ++ NT rx :: gsuf) (productions g)
+      -> In (rx, gamma) (productions g)
+      -> (@derivesForest g) gamma wmid fmid
+      -> (@derivesForest g) gsuf wsuf fsuf
+      -> forall wmid' wsuf' gamma' fmid' fsuf',
+          In (rx, gamma') (productions g)
+          -> (@derivesForest g) gamma' wmid' fmid'
+          -> (@derivesForest g) gsuf wsuf' fsuf'
+          -> word = wmid ++ wsuf
+          -> word = wmid' ++ wsuf'
+          -> wmid = wmid'
+             /\ wsuf = wsuf'
+             /\ gamma = gamma'.
+Proof.
+  intros tbl g Htbl.
+  pose proof Htbl as H.
+  destruct H as [Hmin Hcom].
+  induction word as [| tok toks]; intros.
+  - admit.
+  - destruct wmid as [| mtok mtoks]; simpl in *; subst.
+    + destruct wmid' as [| mtok' mtoks']; simpl in *; subst.
+      * apply derivesForest_nil_nullable in H1.
+        apply derivesForest_nil_nullable in H4.
+        assert (Hlk : (@isLookaheadFor g) EOF (NT rx) gamma).
+        { unfold isLookaheadFor.
+          right.
+          split.
+          - constructor; auto.
+          - constructor; auto.
+            repeat (econstructor; eauto). }
+        assert (Hlk' : (@isLookaheadFor g) EOF (NT rx) gamma').
+        { unfold isLookaheadFor.
+          right.
+          split.
+          - constructor; auto.
+          - constructor; auto.
+            repeat (econstructor; eauto). }
+        unfold ptComplete in Hcom.
+        apply Hcom in Hlk.
+        apply Hcom in Hlk'.
+        destruct Hlk as [laMap [Hsf Hlf]].
+        destruct Hlk' as [laMap' [Hsf' Hlf']].
+        assert (gamma = gamma') by congruence.
+        auto.
+      * (* first/follow conflict *)
+        exfalso.
+        inv H7.
+        admit.
+    + inv H7.
+      destruct wmid' as [| mtok' mtoks'] eqn:Hwm; simpl in *.
+      * (* another first/follow conflict *)
+        admit.
+      * inv H6.
+        inv H9.
+        
+        inv H2; inv H5.
+        
+        eapply IHtoks with
+            (gamma := gamma)
+            (wmid := mtoks)
+            (wsuf0 := wsuf)
+            (wmid' := mtok' :: mtoks')
+            (gamma' := gamma')
+            (wsuf' := wsuf') in H5; eauto.
+        assert (Hlk : (@isLookaheadFor g)
+                        (LA mtok')
+                        (NT rx)
+                        gamma).
+          { unfold isLookaheadFor.
+            right.
+            split.
+            { constructor; auto.
+              apply derivesForest_nil_nullable in H2.
+              auto. }
+            { constructor; auto.
+              eapply FoRight; eauto.
+              apply derivesForest_cons_firstGamma in H3.
+              auto. }}
+          assert (Hlk' : (@isLookaheadFor g)
+                           (LA mtok')
+                           (NT rx)
+                           gamma').
+          { unfold isLookaheadFor.
+            left.
+            constructor; auto.
+            apply derivesForest_cons_firstGamma in H5.
+            auto. }
+          unfold ptComplete in Hcom.
+          apply Hcom in Hlk; apply Hcom in Hlk'.
+          destruct Hlk as [laMap [Hsf Hlf]].
+          destruct Hlk' as [laMap' [Hsf' Hlf']].
+          assert (gamma = gamma') by congruence.
+          subst.
+          assert ((@firstProd g)
+                    (LA mtok')
+                    (NT rx) gamma').
+          { constructor; auto.
+            apply derivesForest_cons_firstGamma in H5.
+            auto. }
+          assert ((@nullableProd g) (NT rx) gamma').
+          { constructor; auto.
+            apply derivesForest_nil_nullable in H2.
+            auto. }
+          assert ((@followProd g)
+                    (LA mtok')
+                    (NT rx) gamma').
+          { constructor; auto.
+            econstructor; eauto.
+            apply derivesForest_cons_firstGamma in H3.
+            auto. }
+          eapply no_first_follow_conflicts; eauto.
+  - destruct wmid' as [| mtok' mtoks']; simpl in *; subst.
+    + (* another first/follow conflict *)
+      exfalso.
+      assert (Hlk : (@isLookaheadFor g)
+                      (LA mtok)
+                      (NT rx)
+                      gamma').
+      { unfold isLookaheadFor.
+        right.
+        split.
+        { constructor; auto.
+          apply derivesForest_nil_nullable in H5.
+          auto. }
+        { constructor; auto.
+          eapply FoRight; eauto.
+          apply derivesForest_cons_firstGamma in H6.
+          auto. }}
+      assert (Hlk' : (@isLookaheadFor g)
+                       (LA mtok)
+                       (NT rx)
+                       gamma).
+      { unfold isLookaheadFor.
+        left.
+        constructor; auto.
+        apply derivesForest_cons_firstGamma in H2.
+        auto. }
+      unfold ptComplete in Hcom.
+      apply Hcom in Hlk; apply Hcom in Hlk'.
+      destruct Hlk as [laMap [Hsf Hlf]].
+      destruct Hlk' as [laMap' [Hsf' Hlf']].
+      assert (gamma = gamma') by congruence.
+      subst.
+      assert ((@firstProd g)
+                (LA mtok)
+                (NT rx) gamma').
+      { constructor; auto.
+        apply derivesForest_cons_firstGamma in H2.
+        auto. }
+      assert ((@nullableProd g) (NT rx) gamma').
+      { constructor; auto.
+        apply derivesForest_nil_nullable in H5.
+        auto. }
+      assert ((@followProd g)
+                (LA mtok)
+                (NT rx) gamma').
+      { constructor; auto.
+        econstructor; eauto.
+        apply derivesForest_cons_firstGamma in H6.
+        auto. }
+      eapply no_first_follow_conflicts; eauto.
+    + inv H7.
+      inv H2.
+      inv H5.
+      subst.
+      apply derivesForest_cons_firstGamma in H0.
+      apply derivesForest_cons_firstGamma in Hderm.
+      assert (Hlk : (@isLookaheadFor g)
+                      (LA mtok')
+                      (NT rx)
+                      gamma).
+      { unfold isLookaheadFor.
+        left.
+        constructor; auto. }
+      assert (Hlk' : (@isLookaheadFor g)
+                       (LA mtok')
+                       (NT rx)
+                       gamma').
+      { unfold isLookaheadFor.
+        left.
+        constructor; auto. }
+      unfold ptComplete in Hcom.
+      apply Hcom in Hlk.
+      apply Hcom in Hlk'.
+      destruct Hlk as [laMap [Hsf Hlf]].
+      destruct Hlk' as [laMap' [Hsf' Hlf']].
+      assert (gamma = gamma') by congruence.
+      auto.
+      subst.
+Qed.
+
+Lemma derives_det :
+  forall tbl g,
+    isParseTableFor tbl g
+    -> forall tr tr' sym word,
+      (@derivesTree g) sym word tr
+      -> (@derivesTree g) sym word tr'
+      -> tr = tr'.
+Proof.
+  intros tbl g Htbl.
+  pose proof Htbl as Htbl'.
+  destruct Htbl as [Hmin Hcom].
+  induction tr using tree_mutual_ind with
+      (P0 := fun fsuf =>
+               forall fsuf' x gpre gsuf
+                      wpre wpre' wsuf wsuf',
+                 In (x, gpre ++ gsuf) (productions g)
+                 -> (@derivesForest g) gsuf wsuf fsuf
+                 -> (@derivesForest g) gsuf wsuf' fsuf'
+                 -> wpre ++ wsuf = wpre' ++ wsuf'
+                 -> wpre = wpre'
+                    /\ wsuf = wsuf'
+                    /\ fsuf = fsuf'); intros.
+
+  - inv H; inv H0; auto.
+
+  - inv H; inv H0.
+    assert (gamma0 = gamma) by admit; subst.
+    eapply IHtr with (gpre := nil) in H2; eauto.
+    destruct H2.
+    destruct H0.
+    subst; auto.
+
+  - inv H0; inv H1.
+    repeat rewrite app_nil_r in *.
+    repeat (split; auto).
+
+  - inv H0; inv H1.
+                     
