LL1/LL1_Derivation.v
@@ -1,0 +1,382 @@
+Require Import List String.
+Require Import Grammar LL1.Parser ParseTree ParseTable
+        Lib.Tactics.
+Import ListNotations.
+Open Scope list_scope.
+
+(* "symbol Sym derives input prefix Pre, producing tree Tr
+    and leaving input suffix Suf unconsumed *)
+Inductive sym_derives_prefix {g : grammar} :
+  symbol -> list string -> tree -> list string -> Prop :=
+| T_sdp : 
+    forall (y : string) (wsuf : list string),
+      sym_derives_prefix (T y) [y] (Leaf y) wsuf
+| NtFirst_sdp :
+    forall (x : string) 
+           (gamma : list symbol)
+           (wpre wsuf : list string) 
+           (subtrees : forest),
+      (@firstProd g) (peek wpre) (NT x) gamma
+      -> gamma_derives_prefix gamma wpre subtrees wsuf
+      -> sym_derives_prefix (NT x) wpre (Node x subtrees) wsuf
+| NtFollow_sdp :
+    forall (x : string) 
+           (gamma : list symbol)
+           (wsuf : list string) 
+           (subtrees : forest),
+      (@followProd g) (peek wsuf) (NT x) gamma
+      -> gamma_derives_prefix gamma [] subtrees wsuf
+      -> sym_derives_prefix (NT x) [] (Node x subtrees) wsuf
+with gamma_derives_prefix {g : grammar} : 
+       list symbol -> list string -> forest -> list string -> Prop :=
+     | Nil_gdp : forall wsuf,
+         gamma_derives_prefix [] [] Fnil wsuf
+     | Cons_gdp : 
+         forall (hdRoot : symbol)
+                (wpre wmid wsuf : list string)
+                (hdTree : tree)
+                (tlRoots : list symbol)
+                (tlTrees : forest),
+         sym_derives_prefix hdRoot wpre hdTree (wmid ++ wsuf)
+         -> gamma_derives_prefix tlRoots wmid tlTrees wsuf
+         -> gamma_derives_prefix (hdRoot :: tlRoots) 
+                                 (wpre ++ wmid)
+                                 (Fcons hdTree tlTrees)
+                                 wsuf.
+            (* Incorrect statement I had before :
+                   gamma_derives_prefix (hdRoots :: tlRoots)
+                                        wpre
+                                        (Fcons hdTree tlTrees)
+                                        (wpre ++ wmid)
+            *)
+
+Scheme sdp_mutual_ind :=
+  Induction for sym_derives_prefix Sort Prop
+  with gdp_mutual_ind :=
+    Induction for gamma_derives_prefix Sort Prop.
+
+Lemma eof_fgamma :
+  forall g la gamma,
+    (@firstGamma g) la gamma
+    -> la = EOF
+    -> False.
+Proof.
+  intros g la gamma H.
+  induction H using firstGamma_mutual_ind with
+      (P := fun la x gamma (pf : firstProd la x gamma) =>
+              la = EOF -> False)
+      (P0 := fun la gamma (pf : firstGamma la gamma) =>
+               la = EOF -> False)
+      (P1 := fun la sym (pf : firstSym la sym) =>
+               la = EOF -> False); intros.
+  - apply IHfirstGamma; trivial.
+  - apply IHfirstGamma; trivial.
+  - apply IHfirstGamma; trivial. 
+  - inv H.
+  - apply IHfirstGamma; trivial.
+Qed.
+
+Lemma nullable_middle_sym :
+  forall g xs ys sym,
+    (@nullableGamma g) (xs ++ sym :: ys)
+    -> (@nullableSym g) sym.
+Proof.
+  induction xs; intros.
+  - simpl in H.
+    inv H.
+    auto.
+  - eapply IHxs.
+    inv H.
+    eauto.
+Qed.
+
+Lemma gamma_with_terminal_not_nullable :
+  forall g xs y zs,
+    (@nullableGamma g) (xs ++ T y :: zs)
+    -> False.
+Proof.
+  induction xs; intros.
+  - simpl in H.
+    inv H.
+  - destruct a.
+    + inv H.
+    + inv H.
+      eapply IHxs; eauto.
+Qed.
+
+Lemma nullable_split :
+  forall g xs ys,
+    (@nullableGamma g) (xs ++ ys)
+    -> (@nullableGamma g) ys.
+Proof.
+  induction xs; intros.
+  - auto.
+  - inv H.
+    eapply IHxs; eauto.
+Qed.
+
+Lemma no_first_follow_conflicts :
+  forall tbl g,
+    isParseTableFor tbl g
+    -> forall la sym,
+      (@firstSym g) la sym
+      -> (@nullableSym g) sym
+      -> (@followSym g) la sym
+      -> False.
+Proof.
+  intros tbl g Htbl la sym Hfi.
+  destruct Htbl as [Hmin Hcom].
+  induction Hfi using firstSym_mutual_ind with
+      (P := fun la sym gamma
+                (pf : (@firstProd g) la sym gamma) =>
+              (@nullableProd g) sym gamma
+              -> (@followSym g) la sym 
+              -> False)
+      (P0 := fun la gammaSuf
+                 (pf : (@firstGamma g) la gammaSuf) =>
+               forall sym gammaPre,
+                 (@firstProd g) la sym (gammaPre ++ gammaSuf)
+                 -> (@nullableProd g) sym (gammaPre ++ gammaSuf)
+                 -> (@followSym g) la sym
+                 -> False)
+      (P1 := fun la sym (pf : (@firstSym g) la sym) =>
+              (@nullableSym g) sym
+              -> (@followSym g) la sym
+              -> False).
+
+  - intros Hnu Hfo.
+    eapply IHHfi; auto.
+    + assert (gamma = [] ++ gamma) by auto.
+      rewrite H in i.
+      econstructor; eauto.
+    + auto.
+    + auto.
+
+  - intros sym gammaPre Hfi' Hnu Hfo.
+    eapply IHHfi.
+    + inv Hnu.
+      apply nullable_middle_sym in H0.
+      auto.
+    + destruct hd.
+      * inv Hnu.
+        apply gamma_with_terminal_not_nullable in H0.
+        inv H0.
+      * inv Hnu.
+        eapply FoLeft; eauto.
+        assert (NT n :: tl = [NT n] ++ tl) by auto.
+        rewrite H1 in H0.
+        rewrite app_assoc in H0.
+        eapply nullable_split in H0.
+        auto.        
+
+  - intros sym gammaPre Hfi Hnu Hfo.
+    eapply IHHfi; eauto.
+    + assert (NT x :: tl = [NT x] ++ tl) by auto.
+      rewrite H in Hfi.
+      rewrite app_assoc in Hfi.
+      eauto.
+    + rewrite <- app_assoc.
+      simpl.
+      auto.
+
+  - intros Hnu Hfo.
+    inv Hfo.
+
+  - intros Hnu Hfo.
+    inv Hnu.
+    inv H.
+    assert (Hlk : (@isLookaheadFor g) la (NT x) gamma).
+    { unfold isLookaheadFor.
+      left.
+      auto. }
+    assert (Hlk' : (@isLookaheadFor g) la (NT x) ys).
+    { unfold isLookaheadFor.
+      right.
+      split.
+      { constructor; auto. }
+      { constructor; auto. }}
+    unfold ptComplete in Hcom.
+    apply Hcom in Hlk; apply Hcom in Hlk'.
+    destruct Hlk as [laMap [Hsf Hlf]].
+    destruct Hlk' as [laMap' [Hsf' Hlf']].
+    assert (gamma = ys) by congruence.
+    subst.
+    apply IHHfi.
+    + constructor; auto.
+    + auto.
+Qed.
+
+Lemma gamma_derives_nil_nullable :
+  forall g gamma wpre f wsuf,
+    (@gamma_derives_prefix g) gamma wpre f wsuf
+    -> wpre = nil
+    -> (@nullableGamma g) gamma.
+Proof.
+  intros g gamma wpre f wsuf Hder.
+  induction Hder using gdp_mutual_ind with
+      (P := fun sym wpre tr wsuf
+                (pf : sym_derives_prefix sym wpre tr wsuf) =>
+              wpre = nil
+              -> nullableSym sym)
+      (P0 := fun gamma wpre f wsuf
+                 (pf : gamma_derives_prefix gamma wpre f wsuf)
+             =>
+               wpre = nil
+               -> nullableGamma gamma); intros; subst.
+  - inv H.
+  - inv f; simpl in *.
+    eapply eof_fgamma in H2; eauto; inv H2.
+  - inv f.
+    econstructor.
+    econstructor; eauto.
+  - constructor.
+  - apply app_eq_nil in H; destruct H; subst.
+    destruct hdRoot as [y | x].
+    + inv s.
+    + econstructor; eauto.
+Qed.
+
+Lemma der_det :
+  forall tbl g,
+    isParseTableFor tbl g
+    -> forall sym wpre wsuf tr,
+      (@sym_derives_prefix g) sym wpre tr wsuf
+      -> forall wpre' wsuf' tr',
+        (@sym_derives_prefix g) sym wpre' tr' wsuf'
+        -> wpre ++ wsuf = wpre' ++ wsuf'
+        -> wpre = wpre' /\ wsuf = wsuf' /\ tr = tr'.
+Proof.
+  intros tbl g Htbl sym wpre wsuf tr Hder.
+  induction Hder using sdp_mutual_ind with
+      (P := fun sym wpre tr wsuf
+                (pf : sym_derives_prefix
+                        sym wpre tr wsuf) =>
+              forall wpre' wsuf' tr',
+                sym_derives_prefix sym wpre' tr' wsuf'
+                -> wpre ++ wsuf = wpre' ++ wsuf'
+                -> wpre = wpre' /\ wsuf = wsuf' /\ tr = tr')
+      (P0 := fun gamma wpre f wsuf
+                 (pf : gamma_derives_prefix gamma wpre f wsuf) =>
+               forall wpre' wsuf' f',
+                 gamma_derives_prefix gamma wpre' f' wsuf'
+                 -> wpre ++ wsuf = wpre' ++ wsuf'              
+                 -> wpre = wpre' /\ wsuf = wsuf' /\ f = f'); intros.
+  - inv H; inv H0; auto.
+    
+  - (* NtFirst case *)
+    inv H.
+    + destruct wpre as [| ptok ptoks]; simpl in *.
+      * inv f.
+        eapply eof_fgamma in H5; eauto; inv H5.
+      * destruct wpre' as [| ptok' ptoks']; simpl in *.
+        -- inv H2.
+           eapply eof_fgamma in H5; eauto; inv H5.
+        -- inv H0.
+           assert (gamma0 = gamma).
+           { destruct Htbl as [Hmin Hcom].
+             unfold ptComplete in Hcom.
+             assert ((@isLookaheadFor g) (LA ptok')
+                                         (NT x)
+                                         gamma).
+             { unfold isLookaheadFor; auto. }
+             assert ((@isLookaheadFor g) (LA ptok')
+                                         (NT x)
+                                         gamma0).
+             { unfold isLookaheadFor; auto. }
+             apply Hcom in H.
+             destruct H as [m [Hs Hl]].
+             apply Hcom in H0.
+             destruct H0 as [m' [Hs' Hl']].
+             congruence. }
+           subst.
+           eapply IHHder in H3; eauto.
+           ++ destruct H3.
+              destruct H0.
+              subst.
+              apply app_inv_tail in H4.
+              auto.
+           ++ rewrite <- app_comm_cons.
+              rewrite H4.
+              auto.
+    + destruct wpre as [| ptok ptoks]; simpl in *.
+      * inv f.
+        eapply eof_fgamma in H5; eauto; inv H5.
+      * destruct wsuf' as [| stok' stoks']; simpl in *.
+        -- inv H0.
+        -- inv H0.
+           assert ((@firstSym g) (LA stok') (NT x)) by
+               (econstructor; eauto).
+           assert ((@nullableSym g) (NT x)).
+           {  inv H2.
+             econstructor.
+             econstructor; eauto.
+             eapply gamma_derives_nil_nullable in H3; eauto. }
+           assert ((@followSym g) (LA stok') (NT x)).
+           { inv H2; auto. }
+           eapply no_first_follow_conflicts in H; eauto.
+           inv H.
+  - (* NtFollow case *)
+    simpl in *.
+    inv H; simpl in *.
+    + destruct wpre' as [| ptok' ptoks']; simpl in *.
+      * inv H2.
+        eapply eof_fgamma in H4; eauto; inv H4.
+      * assert ((@firstSym g) (LA ptok') (NT x)) by
+               (econstructor; eauto).
+        assert ((@nullableSym g) (NT x)).
+        { inv f.
+          econstructor.
+          econstructor; eauto.
+          eapply gamma_derives_nil_nullable in g0; eauto. }
+        assert ((@followSym g) (LA ptok') (NT x)).
+        { inv f; auto. }
+        eapply no_first_follow_conflicts in H; eauto.
+        inv H.
+    + assert (gamma0 = gamma).
+      { destruct Htbl as [Hmin Hcom].
+        unfold ptComplete in Hcom.
+        assert ((@isLookaheadFor g) (peek wsuf')
+                                    (NT x)
+                                    gamma).
+        { unfold isLookaheadFor.
+          right.
+          split.
+          - inv f.
+            constructor; auto.
+            eapply gamma_derives_nil_nullable in g0; eauto.
+          - auto. }
+        assert ((@isLookaheadFor g) (peek wsuf')
+                                    (NT x)
+                                    gamma0).
+        { unfold isLookaheadFor.
+          right.
+          split.
+          - inv H2.
+            constructor; auto.
+            eapply gamma_derives_nil_nullable in H3; eauto.
+          - auto. }
+        apply Hcom in H.
+        destruct H as [m [Hs Hl]].
+        apply Hcom in H0.
+        destruct H0 as [m' [Hs' Hl']].
+        congruence. }
+      subst.
+      eapply IHHder in H3; eauto.
+      destruct H3.
+      destruct H0.
+      subst; auto.
+
+  - inv H; auto.
+
+  - inv H.
+    eapply IHHder in H3; eauto.
+    + destruct H3.
+      destruct H1; subst.
+      eapply IHHder0 in H7; eauto.
+      destruct H7.
+      destruct H2.
+      subst; auto.
+    + repeat rewrite app_assoc; auto.
+Qed. (* Finally! *)            
+
+    
